%!TEX root = main.tex

\section{A Propagation-Based Calculus}
\label{sect:calculus}

\begin{table}
  \begin{gather*}
    \infer
    {\seqq{\phi \wedge \psi}}
    {\seqq{\phi, \psi}}
    \qquad
    \infer
    {\seqq{ \neg(\phi \vee \psi)}}
    {\seqq{ \neg\phi, \neg\psi}}
    \qquad
    \infer
    {\seqq{\phi \vee \psi}}
    {\seqq{\phi} & \seqq{\psi}}
    \qquad
    \infer
    {\seqq{\neg(\phi \wedge \psi)}}
    {\seqq{\neg\phi} & \seqq{\neg\psi}}
    \qquad
    \infer
    {\seqq{ \neg\neg\phi}}
    {\seqq{\phi}}
    \\
    \infer
    {\seqq{x \not\in e}}
    {\seqq{x \in e^C}}
    \qquad
    \infer[\text{where~} y \text{~is fresh}]
    {\seqq{x \not= f(x_1, \ldots, x_n)}}
    {\seqq{x \not= y, y = f(x_1, \ldots, x_n)}}
    \qquad
    \infer
    {\seqq{}}
    {\seqq{x \in e} & \seqq{x \in e^C}}
    \\[2ex]
    \infer[\text{if~} \lang{e_1} \cap \cdots \cap\lang{e_1} = \emptyset]
    {\seqq{x \in e_1, \ldots, x \in e_n}}
    {*}
    \\
    \infer[\text{if~} \lang{e_1} \cap \cdots \cap\lang{e_1} \subseteq \lang{e}]
    {\seqq{x \in e, x \in e_1, \ldots, x \in e_n}}
    {\seqq{x \in e_1, \ldots, x \in e_n}}
    \\
    \infer[\text{if~} n > 1 \text{~and~} \lang{e_1} \cap \cdots \cap\lang{e_1} = \lang{e}]
    {\seqq{x \in e_1, \ldots, x \in e_n}}
    {\seqq{x \in e}}
    \\[2ex]
    \infer
    {\seqq{x \in e, x = y}}
    {\seqq{x \in e, x = y, y \in e}}
    \qquad
    \infer[\text{if~} |\lang{e}| = 1]
    {\seqq{x \in e, x \not= y}}
    {\seqq{x \in e, x \not= y, y \in e^C}}
    \\
    \infer[\text{if~} \lang{e_1} \cap \lang{e_2} = \emptyset]
    {\seqq{x \in e_1, x \not= y, y \in e_2}}
    {\seqq{x \in e_1, y \in e_2}}
    \\[2ex]
    \infer[\text{if~} \lang{e} = f(\lang{e_1}, \ldots, \lang{e_n})]
    {\seqq{x = f(x_1, \ldots, x_n), x_1 \in e_1, \ldots, x_n \in e_n}}
    {\seqq{x \in e, x = f(x_1, \ldots, x_n), x_1 \in e_1, \ldots, x_n \in e_n}}
    \\
    \infer[\text{if~}
    \begin{array}{l}
      \lang{e} = f(\lang{e_1}, \ldots, \lang{e_n}),
      \\
      |\lang{e_1}| = \cdots = |\lang{e_n}| = 1
    \end{array}]
    {\seqq{x = f(x_1, \ldots, x_n), x_1 \in e_1, \ldots, x_n \in e_n}}
    {\seqq{x \in e, x_1 \in e_1, \ldots, x_n \in e_n}}
    \\
    \infer[\text{if~}
    \bigcup_{i=1}^k \big( \lang{e_1^i} \times \cdots \times \lang{e_n^i} \big) =
    f^{-1}(\lang{e})]
    {\seqq{x \in e, x = f(x_1, \ldots, x_n)}}
    {\big\{\seqq{x \in e, x = f(x_1, \ldots, x_n),
        x_1 \in e_1^i, \ldots, x_n \in e_n^i}\big\}_{i=1}^k}
  \end{gather*}
  
  \caption{Rules of the one-sided sequent calculus}
\end{table}


%%% Local Variables:
%%% mode: latex
%%% TeX-master: "main"
%%% TeX-command-extra-options: "-shell-escape"
%%% End:
